Registers.thy
@@ -1,0 +1,46 @@
+theory Registers
+  imports Definitions
+begin
+
+section "Simps"
+
+lemma memory_\<alpha>_eq[simp]: "memory_\<alpha> (vs,s,h) = memory_\<alpha> (vs',s,h)"
+  apply (rule ext)
+  subgoal for x
+    by (cases x; simp)
+  done
+
+lemma register_\<alpha>_update_eq[simp]:
+  "register_\<alpha> (Mapping.update n v vs, s, h) = (register_\<alpha> (vs, s, h))(reg n := Some v)"
+  apply (auto simp: fun_eq_iff split: llvm_value_ref.split)
+  subgoal for x by (cases x; simp)
+  done
+
+
+section "Lemmas"
+
+named_theorems register_intro
+
+lemma wp_set_register_value_intro[THEN consequence, register_intro]:
+  "wp (return (set_register_value vs n v,s,h)) (\<lambda>s'. register_\<alpha> s' = (register_\<alpha> (vs,s,h))(reg n := Some v) \<and> memory_\<alpha> s' = memory_\<alpha> (vs,s,h))"
+  unfolding set_register_value_def
+  by (intro wp_intro wp_return_intro; simp)
+
+lemma wp_set_register_intro[THEN consequence, wp_intro]:
+  shows "wp (return (set_register s n v)) (\<lambda>s'. register_\<alpha> s' = (register_\<alpha> s)(reg n := Some v) \<and> memory_\<alpha> s' = memory_\<alpha> s)"
+  by (cases s; simp; intro wp_intro register_intro; simp)
+
+
+lemma wp_get_register_value_intro[THEN consequence, register_intro]:
+  assumes "register_\<alpha> (vs,s,h) (reg n) = Some v"
+  shows "wp (get_register_value vs n) (\<lambda>v'. v' = v)"
+  using assms
+  by (induction vs; simp; intro wp_intro; simp add: option.case_eq_if split: if_splits)
+
+lemma wp_get_register_intro[THEN consequence, wp_intro]:
+  assumes "register_\<alpha> s n = Some v"
+  shows "wp (get_register s n) (\<lambda>v'. v' = v)"
+  using assms
+  by (cases s; cases n; simp; intro register_intro; simp)
+
+end
